lang/LangTest.v
@@ -420,7 +420,7 @@ Module MultiCore.
 
   Definition programs: list Lang.program :=
     [program (Int.repr 0) ; program (Int.repr 10); program (Int.repr 20)].
-
+  
 End MultiCore.
 
 
